
\documentclass{article}
\usepackage[utf8]{inputenc}
\usepackage{graphicx}
\usepackage{epstopdf}
\usepackage{amsmath}
\usepackage{xcolor}
\usepackage[ruled]{algorithm2e} 

\newcommand{\R}{\mathbb{R}} 

\title{The BTL Model}
\author{Xiaolin Shen}

\begin{document}

\maketitle


\section{The Standard BTL Model}

Suppose that there are $K$ underlying aspects, the latent preference vector for each user is denoted as $ u \in  R+ ^K$ , and $\sum_k u_k = 1$ , latent item feature vector $ i, j \in R +^K$.

Base on the standard BTL model:

\begin{align*}
	p(i \succ j |u)=\frac{u^{T}i}{u^{T}i+ u^{T}j} \\
	p(i \prec j |u)=1-p(i \succ j |u)
\end{align*}

We use the maximal likelihood estimation. The likelihood function can be written as follows. The model parameters are denoted as $ \Theta = \{ v \in V ,u \in U \}$, $\succ_d $ represents a pairwise ranking observation in a session $d$.
\begin{align}
L(\Theta)
= \Pi_{d \in D} \Pi_{i \succ_d j}\frac{\sum_{k=1}^{K} u_k i_k}{\sum_{k=1}^{K} u_k i_k+ \sum_{k=1}^{K} u_k j_k}
\end{align}

Thus, the log likelihood and its lower bound is:
\begin{align}
l(\Theta) &= \log \; L(\Theta) \\
& =\sum_{u} \sum_{d\in D_u} \sum_{i \succ_d j} \log \;  \frac{\sum_k u_k i_k}{\sum_k u_k i_k+ \sum_k u_k j_k}\\ \nonumber
& \geq \sum_{u} \sum_{d\in D_u} \sum_{i \succ_d j}[1- \frac{\sum_k u_k i_k+ \sum_k u_k j_k}{\sum_k u_k^t i_k^t+ \sum_k u_k^t j_k^t}+ \log \frac{\sum_k u_k i_k}{\sum_k u_k^t i_k^t+ \sum_k u_k^t j_k^t}]
\end{align}
where we apply
\begin{equation*}
\ln \frac{y}{x} \geq 1- \frac{x}{y}
\end{equation*}

To maximize the lower-bound in $Equ.3$ we employ conjugate gradient method.

We first fix all latent vectors for the item $\footnote{We use the supscript $t$ for parameters in the $t^{th}$ round}$, and apply  $ \log \sum_k u_k i_k \geq \frac{\sum_k i_k \log u_k}{\sum_k i_k} + \log \sum_k i_k,\forall i_k \geq 0.$ Let's compute $c^t(d,i,j)=\sum_k u_k^ti_k^t + \sum_k u_k^tj_k^t$, $c_k^t(d,i,j)=\frac{i_k^t + j_k^t}{c^t(d,i,j)}$, and $ f_k^t(d,i)=\frac{i_k^t}{\sum_k i_k^t} $ for all pairwise ranking observations in $d$ using the $t$-th round parameters, we have  
\begin{align}
\frac{\partial \;l }{\partial \;u_k}
 &=\sum_{d\in D_u} \sum_{i \succ_d j} (\frac{f_k^t(d,i)}{u_k} - c_k^t(d,i,j) ) =0\\
\end{align}

Here we omit the constraint that $u_k \geq 0$ and hope that this constraint will be satisfied by the solution.
\begin{align}
u_k = \frac{\sum_{d\in D_u} \sum_{i \succ_d j} \frac{i_k}{\sum_k i_k} }{\sum_{d\in D_u} \sum_{i \succ_d j}\frac{i_k+j_k}{c^t(i,j,d)}}
\end{align}


Next we fix all user latent vectors, and again apply the Jensenâ€™s inequality $\log \sum_k u_k i_k \geq \frac{\sum_k u_k \log i_k}{\sum_k u_k}+ \log \sum_k u_k,\forall u_k \geq 0$.  For convenience, we use $v$  to denote a arbitral item, and $O_u$  is the set of all observed pairwise ranking of user u, if $ v \succ j $ is the winning item then we say $o \in W(v)$.  We first compute $e_k^t(u) = \frac{u_k^t}{\sum_k u_k^t}$

\begin{align}
\frac{\partial \;l}{\partial \;v_k}
 &=\sum_{u} \sum_{o \in W(v) \&\& o \in O_u} \frac{e_k^t(u)}{v_k} - \sum_{u} \sum_{o \in O_u,i=v||j=v} \frac{u_k}{c^t(i, j, d)} =0\\
 & v_k =\frac{\sum_{u} \sum_{o \in W(v) \&\& o \in O_u} e_k^t(u)}{\sum_{u} \sum_{o \in O_u,i=v||j=v} \frac{u_k}{c^t(i, j, d)}}
\end{align}

Again we omit the constraint that $v_k \geq 0$ because that is satisfied automatically by the solution. We have to renormalize $\forall k, \sum_v v_k =1 $.

\begin{algorithm}[H]
    \caption{Standard BTL Algorithm}
    \KwIn{A set of pairwise rankings $D$, number of aspects $K$, maximal number of iterations $MaxIter$}
    \KwOut{$U,V$ }

    initialization: Randomize $U,V$, $\forall k, u_k\geq 0, v_k \geq 0, \sum_v v_k=1$ \;
    \For {$t=1; t\leq MaxIter; t++$}{
        Randomize order of observations \;
        \For{$u\in U$}{
        $c^t(d,i,j)=\sum_k u_k^t i_k^t + \sum_k u_k^t j_k^t, f^t(d,i)=\sum_k i_k^t $\;
        \For{$k=1;k\leq K,k++$}{
        $c_k^t(d,i,j)=\frac{i_k^t + j_k^t}{c^t(d,i,j)}, f_k^t(d,i)=\frac{i_k^t}{f^t(d,i)}$\;
        }
        $u_k^{t+1}= \frac{\sum_{d \in D_u} \sum_{i\succ_d j }  f_k^t(d,i) }{ \sum_{d \in D_u} \sum_{i\succ_d j } c_k^t(d,i,j)}$\;
        }
    \For{$v\in V$}{
        $e^t(u)=\sum_k u_k^t$\;
        \For{$k=1;k\leq K,k++$}{
        $e_k^t(u)=\frac{u_k^t}{e^t(u)}$\;
        }
        $v_k= \frac{\sum_u \sum_{o \in W(v) \&\& o\in O_u}  e_k^t(u)}{ \sum_u \sum_{o \in O_u, i=v\| j=v} \frac{u_k}{c^t(i,j,d)}}$\;
        }
}
\end{algorithm}

\end{document}
